src/dice/DICE.Definitions.fst
@@ -8,11 +8,22 @@ module B = LowStar.Buffer
 module S = Spec.Hash.Definitions
 module H = Hacl.Hash.Definitions
 
+open Lib.IntTypes
+
 (*
  * Some common definitions used in the DICE code
  *)
 
 #set-options "--__temp_no_proj DICE.Definitions"
+
+let byte_sec = uint8
+let byte_pub = pub_uint8
+
+let bytes_sec = Seq.seq I.uint8
+let bytes_pub = Seq.seq I.pub_uint8
+
+let lbytes_sec = Seq.lseq I.uint8
+let lbytes_pub = Seq.lseq I.pub_uint8
 
 type dice_hash_alg = a:S.hash_alg{a =!= S.MD5 /\ a =!= S.SHA2_224}
 
@@ -39,8 +50,8 @@ unfold let digest_len = H.hash_len alg
 
 unfold type digest_t = H.hash_t alg
 
-unfold type hashable_len = i:I.size_t{0 < I.v i /\ I.v i <= S.max_input_length alg}
-
+unfold type hashable_len = i: size_t {0 < v i /\ v i <= S.max_input_length alg}
+unfold type signable_len = i: size_t {64 + v i <= max_size_t}
 unfold let cdi_len = digest_len
 
 
@@ -49,30 +60,65 @@ unfold let cdi_len = digest_len
 unfold type signature_t = B.lbuffer I.uint8 64
 unfold type key_t = B.lbuffer I.uint8 32
 
-
 noeq
-type riot_header_t = {
-  binary_size : hashable_len;
-  header_sig  : signature_t;  //signature of the hash of the binary
-  
-  binary      : B.lbuffer I.uint8 (I.v binary_size);
-  pubkey      : (k:key_t{
-    B.(all_disjoint [
-        B.loc_buffer header_sig;
-        B.loc_buffer binary;
-        B.loc_buffer k ])
-  });
-}
+type image_t = {
+  header_size : signable_len;
+  image_header: B.lbuffer byte_sec (v header_size);
+  image_hash  : digest_t;
+  header_sig  : signature_t;
+  image_size  : hashable_len;
+  image_base  : image_base: B.buffer byte_sec
+                { B.length image_base == v image_size };
+(* NOTE: This pubkey is not part of the image *)
+  pubkey      : pubkey: key_t
+                { B.all_disjoint [B.loc_buffer image_header;
+                                  B.loc_buffer image_hash;
+                                  B.loc_buffer header_sig;
+                                  B.loc_buffer image_base;
+                                  B.loc_buffer pubkey] }
+  }
 
-let riot_header_locs (rh:riot_header_t) : GTot (list B.loc) = [
-  B.loc_buffer rh.header_sig;
-  B.loc_buffer rh.binary;
-  B.loc_buffer rh.pubkey
-]
-
-let contains_riot_header (h:HS.mem) (rh:riot_header_t) =
+let contains_image (h:HS.mem) (image:image_t) =
   B.all_live h [
-    B.buf rh.header_sig;
-    B.buf rh.binary;
-    B.buf rh.pubkey
+    B.buf image.header_sig;
+    B.buf image.image_header;
+    B.buf image.image_hash;
+    B.buf image.image_base;
+    B.buf image.pubkey
   ]
+
+let locs_of_image (image: image_t) =
+  [B.loc_buffer image.image_header;
+   B.loc_buffer image.image_hash;
+   B.loc_buffer image.header_sig;
+   B.loc_buffer image.image_base;
+   B.loc_buffer image.pubkey]
+
+open Lib.ByteBuffer
+module S = Spec.Hash.Definitions
+module Ed25519 = Hacl.Ed25519
+
+let is_valid_image
+  (pubkey: lbytes_sec 32)
+  (image: bytes_sec {0 < Seq.length image /\ Seq.length image <= S.max_input_length alg})
+  (image_hash: lbytes_sec 32)
+  (image_header: bytes_sec {Seq.length image_header + 64<= max_size_t})
+  (header_sig: lbytes_sec 64)
+: Type0
+= Spec.Ed25519.verify
+    (* key *) pubkey
+    (* msg *) image_header
+    (* sig *) header_sig /\
+  image_hash == Spec.Agile.Hash.hash alg image
+
+let is_valid_image_st
+  (image: image_t)
+  (h: HS.mem)
+: Type0
+= Spec.Ed25519.verify
+    (* key *) (B.as_seq h image.pubkey)
+    (* msg *) (B.as_seq h image.image_header)
+    (* sig *) (B.as_seq h image.header_sig) /\
+  B.as_seq h image.image_hash ==
+  Spec.Agile.Hash.hash alg
+    (* msg *) (Seq.slice (B.as_seq h image.image_base) 0 (v image.image_size))
