src/dice/HWAbstraction.fst
@@ -7,52 +7,124 @@ module HS = FStar.HyperStack
 module HST = FStar.HyperStack.ST
 
 module B = LowStar.Buffer
+module IB = LowStar.ImmutableBuffer
 
 let uds_len = 0x20ul
+let uds_value = fun _ -> Seq.create (v uds_len) (u8 0)
+let uds_buf = IB.igcmalloc HS.root (u8 0) uds_len
 
-#set-options "--max_fuel 0 --ifuel 2 --__temp_no_proj HWAbstraction"
+let riot_pubkey_value = fun _ -> Seq.create 32 (u8 0)
+let riot_pubkey_buf = IB.igcmalloc HS.root (u8 0) 32ul
 
-noextract
-type t =
-  | Uninitialized
-  | Enabled
-  | Disabled
+let image_size = 1ul
+let riot_image_value = fun _ -> Seq.create (v image_size) (u8 0)
+let riot_image_buf = IB.igcmalloc HS.root (u8 0) image_size
+
+let riot_image_hash_value = fun _ -> Seq.create 32 (u8 0)
+let riot_image_hash_buf = IB.igcmalloc HS.root (u8 0) 32ul
+
+let header_size = 100ul
+let riot_image_header_value = fun _ -> Seq.create (v header_size) (u8 0)
+let riot_image_header_buf = IB.igcmalloc HS.root (u8 0) header_size
+
+let riot_header_sig_value = fun _ -> Seq.create 64 (u8 0)
+let riot_header_sig_buf = IB.igcmalloc HS.root (u8 0) 64ul
+
+#set-options "--__temp_no_proj HWAbstraction"
+
+let stack_is_zeroized h =
+  G.reveal (HS.sel h hwi_state) == Zeroized
+
+let uds_is_disabled h =
+  G.reveal (HS.sel h hwi_state) == Disabled
+
+let get_riot_image () buf_disj
+= (* Prf *) HST.recall hwi_state; (* Recall for disjointness *)
+  let pubkey = B.alloca (u8 0x00) 32ul in
+  // (* Prf *) let h = HST.get () in
+  // (* Prf *) IB.recall riot_pubkey_buf;
+  // (* Prf *) IB.recall_contents riot_pubkey_buf (Seq.create 32 (u8 0));
+  // (* Prf *) IB.buffer_immutable_buffer_disjoint pubkey riot_pubkey_buf h;
+  // B.blit riot_pubkey_buf 0ul pubkey 0ul 32ul;
+  let image_base = B.alloca (u8 0x00) image_size in
+  let image_hash = B.alloca (u8 0x00) 32ul in
+  let image_header = B.alloca (u8 0x00) header_size in
+  let header_sig = B.alloca (u8 0x00) 64ul in
+  { header_size = header_size;
+    image_header = image_header;
+    image_hash = image_hash;
+    header_sig = header_sig;
+    image_size = image_size;
+    image_base = image_base;
+    pubkey = pubkey }
+
+#push-options "--z3rlimit 16 --fuel 0 --ifuel 0"
+let read_uds uds
+= HST.recall hwi_state;
+  HST.(hwi_state := Copied);
+  B.fill uds (u8 0x00) uds_len
+#pop-options
+
+let platform_zeroize_stack ()
+= HST.recall hwi_state;
+  HST.(hwi_state := Zeroized)
+
+let disable_uds ()
+= HST.recall hwi_state;
+  HST.(hwi_state := Disabled)
+  // HST.witness_p local_state_ref uds_is_copied_predicate
+
+let platform_zeroize len b
+= B.fill b (u8 0) len;
+  let h1 = HST.get () in
+  Seq.lemma_split (B.as_seq h1 b) (v len)
 
 
-let t_rel : P.preorder (G.erased t) =
-  fun x1 x2 ->
-  match (G.reveal x1, G.reveal x2) with
-  | Uninitialized, _
-  | Enabled, Disabled -> True
-  | _, _ -> x1 == x2
+(* Old implemenations
+let initialize () =
+  HST.recall local_state_ref;
+  HST.(local_state_ref := Enabled);
+  HST.witness_p local_state_ref uds_is_initialized_predicate;
+
+  let uds = B.malloc HS.root (u8 0x00) uds_len in
+  let cdi = B.malloc HS.root (u8 0x00) cdi_len in
+
+  let binary_size = 1ul in
+  let header_sig = B.malloc HS.root (u8 0x00) 64ul in
+  let binary = B.malloc HS.root (u8 0x00) 1ul in
+  let pubkey = B.malloc HS.root (u8 0x00) 32ul in
+
+  let riot_header = {
+    binary_size = binary_size;
+    header_sig = header_sig;
+    binary = binary;
+    pubkey = pubkey
+  } in
+
+  let uds_seq =
+    let h = HST.get () in
+    G.hide (B.as_seq h uds) in
+
+  { uds = uds;
+    cdi = cdi;
+    riot_header = riot_header;
+    uds_val = uds_seq }
+
+let unset_uds st =
+  let uds = get_uds st in
+  B.fill uds (u8 0x00) uds_len;
+  let h = HST.get () in
+  assert (Seq.equal (B.as_seq h uds) (Seq.create (v uds_len) (u8 0x00)))
+
+let disable_uds st =
+  HST.recall_p local_state_ref uds_is_initialized_predicate;
+  HST.(local_state_ref := Disabled);
+  HST.witness_p local_state_ref uds_is_disabled_predicate;
+
+  B.free st.uds
 
 
-let local_state_ref : HST.mref (G.erased t) t_rel = HST.ralloc HS.root (G.hide Uninitialized)
-
-
-let local_state = (| t, t_rel,  local_state_ref |)
-
-
-let uds_is_uninitialized h =
-  G.reveal (HS.sel h local_state_ref) == Uninitialized
-
-
-let uds_is_initialized_predicate : HST.mem_predicate =
-  fun h ->
-  let x = G.reveal (HS.sel h local_state_ref) in
-  x == Enabled \/ x == Disabled
-
-
-let uds_is_initialized = HST.token_p local_state_ref uds_is_initialized_predicate
-
-
-let uds_is_disabled_predicate : HST.mem_predicate =
-  fun h -> G.reveal (HS.sel h local_state_ref) == Disabled
-
-
-let uds_is_disabled = HST.token_p local_state_ref uds_is_disabled_predicate
-
-
+(* Old Implementation
 noeq
 type state = {
   uds : B.buffer uint8;
