src/dice/DICE.Test.fst
@@ -1,0 +1,33 @@
+module DICE.Test
+
+open LowStar.Comment
+
+module Fail = LowStar.Failure
+module B = LowStar.Buffer
+module HS  = FStar.HyperStack
+module HST = FStar.HyperStack.ST
+
+open Lib.IntTypes
+open Lib.ByteBuffer
+module S = Spec.Hash.Definitions
+module Ed25519 = Hacl.Ed25519
+
+module HW = HWAbstraction
+
+open DICE.Definitions
+open DICE.Core
+
+let main ()
+: HST.ST C.exit_code
+  (requires fun h -> HW.uds_is_enabled h)
+  (ensures fun _ _ _ -> True)
+= HST.push_frame ();
+
+  (* Prf *) HST.recall HW.hwi_state; (* for liveness *)
+
+  let cdi: B.lbuffer byte_sec (v digest_len) = B.alloca (u8 0x00) digest_len in
+
+  let ret = dice_main cdi in
+
+  HST.pop_frame ();
+  C.EXIT_SUCCESS
